examples/sbf/verif_Ingress.v
@@ -19,8 +19,16 @@ Import ListNotations.
 
 Definition ipv4_header : Type := Z * Z.
 
-Definition is_internal (ip_addr : Z) : bool.
-Admitted.
+Definition ipv4_addr_w := 32%N.
+
+(* This is kind of cheating. :) *)
+Definition is_internal (ip_addr : Z) : bool :=
+  (Tofino.values_match_mask
+         (ValBaseBit (P4Arith.to_lbool ipv4_addr_w ip_addr))
+         (eval_p4int_val
+            {| tags := NoInfo; value := 2154823680; width_signed := None |})
+         (eval_p4int_val
+            {| tags := NoInfo; value := 4294901760; width_signed := None |})).
 
 (* The bool in the return value means the packet is allowed. *)
 Definition process (f : filter) '((timestamp, ipv4) : Z * ipv4_header) : filter * option bool :=
@@ -28,11 +36,309 @@ Definition process (f : filter) '((timestamp, ipv4) : Z * ipv4_header) : filter 
     (filter_insert f (timestamp, ipv4), Some true)
   else
     (filter_clear f timestamp,
-      filter_query (filter_clear f timestamp) (timestamp, (snd ipv4, fst ipv4))).
+      option_map negb (filter_query (filter_clear f timestamp) (timestamp, (snd ipv4, fst ipv4)))).
 
 Definition p := ["pipe"; "ingress"].
 
-Definition ipv4_addr_w := 32%N.
+Definition act_for_tbl_1_action_0_fd :=
+  ltac:(get_fd ["SwitchIngress"; "act_for_tbl_1_action_0"] ge).
+
+Definition act_for_tbl_1_action_0_spec :=
+  WITH (* p *),
+    PATH p
+    MOD (Some [["ig_md"]]) []
+    WITH ,
+      PRE
+        (ARG []
+        (MEM [(["ig_md"], force ValBaseNull (uninit_sval_of_typ None metadata_t))]
+        (EXT [])))
+      POST
+        (ARG_RET [] ValBaseNull
+        (MEM [(["ig_md"], update "solicited" (P4Bit 8 0)
+          (force ValBaseNull (uninit_sval_of_typ None metadata_t)))]
+        (EXT []))).
+
+Lemma act_for_tbl_1_action_0_body :
+  func_sound ge act_for_tbl_1_action_0_fd nil act_for_tbl_1_action_0_spec.
+Proof.
+  start_function.
+  step.
+  step.
+  entailer.
+Qed.
+
+Definition tbl_for_stmt_1_fd :=
+  ltac:(get_fd ["SwitchIngress"; "tbl_for_stmt_1"; "apply"] ge).
+
+Definition tbl_for_stmt_1_spec :=
+  WITH (* p *),
+    PATH p
+    MOD (Some [["ig_md"]]) []
+    WITH ,
+      PRE
+        (ARG []
+        (MEM [(["ig_md"], force ValBaseNull (uninit_sval_of_typ None metadata_t))]
+        (EXT [])))
+      POST
+      (EX retv,
+        (ARG_RET [] retv
+        (MEM [(["ig_md"], update "solicited" (P4Bit 8 0)
+          (force ValBaseNull (uninit_sval_of_typ None metadata_t)))]
+        (EXT []))))%arg_ret_assr.
+
+Lemma tbl_for_stmt_1_body :
+  func_sound ge tbl_for_stmt_1_fd nil tbl_for_stmt_1_spec.
+Proof.
+  start_function.
+  table_action act_for_tbl_1_action_0_body.
+  { entailer. }
+  { entailer. }
+Qed.
+
+#[local] Hint Extern 5 (func_modifies _ _ _ _ _) => (apply tbl_for_stmt_1_body) : func_specs.
+
+Definition bf2_act_set_insert_key_fd :=
+  ltac:(get_fd ["SwitchIngress"; "bf2_act_set_insert_key"] ge).
+
+Definition bf2_act_set_insert_key_spec :=
+  WITH (* p *),
+    PATH p
+    MOD (Some [["ig_md"]; ["bf2_act_set_insert_key"; "api"]]) []
+    WITH h,
+      PRE
+        (ARG [P4Bit 8 INSERT]
+        (MEM [(["hdr"], update "ipv4"
+                (update "src_addr" (P4Bit ipv4_addr_w (fst h))
+                  (update "dst_addr" (P4Bit ipv4_addr_w (snd h))
+                    (force ValBaseNull (uninit_sval_of_typ (Some true) ipv4_h))))
+                (force ValBaseNull (uninit_sval_of_typ None header_t)));
+              (["ig_md"], update "solicited" (P4Bit 8 0)
+                (force ValBaseNull (uninit_sval_of_typ None metadata_t)))]
+        (EXT [])))
+      POST
+        (ARG_RET [] ValBaseNull
+        (MEM [(["ig_md"], update "bf2_key" (eval_val_to_sval (ValBaseBit
+                (P4Arith.to_lbool ipv4_addr_w (fst h) ++ P4Arith.to_lbool ipv4_addr_w (snd h))))
+          (update "bf2_api" (P4Bit 8 INSERT)
+            (update "solicited" (P4Bit 8 0)
+              (force ValBaseNull (uninit_sval_of_typ None metadata_t)))))]
+        (EXT []))).
+
+Lemma bf2_act_set_insert_key_body : 
+  func_sound ge bf2_act_set_insert_key_fd nil bf2_act_set_insert_key_spec.
+Proof.
+  start_function.
+  step.
+  step.
+  step.
+  entailer.
+Qed.
+
+#[local] Hint Extern 5 (func_modifies _ _ _ _ _) => (apply bf2_act_set_insert_key_body) : func_specs.
+
+Definition bf2_act_set_query_key_fd :=
+  ltac:(get_fd ["SwitchIngress"; "bf2_act_set_query_key"] ge).
+
+Definition bf2_act_set_query_key_spec :=
+  WITH (* p *),
+    PATH p
+    MOD (Some [["ig_md"]; ["bf2_act_set_query_key"; "api"]]) []
+    WITH h,
+      PRE
+        (ARG [P4Bit 8 QUERY]
+        (MEM [(["hdr"], update "ipv4"
+                (update "src_addr" (P4Bit ipv4_addr_w (fst h))
+                  (update "dst_addr" (P4Bit ipv4_addr_w (snd h))
+                    (force ValBaseNull (uninit_sval_of_typ (Some true) ipv4_h))))
+                (force ValBaseNull (uninit_sval_of_typ None header_t)));
+              (["ig_md"], update "solicited" (P4Bit 8 0)
+                (force ValBaseNull (uninit_sval_of_typ None metadata_t)))]
+        (EXT [])))
+      POST
+        (ARG_RET [] ValBaseNull
+        (MEM [(["ig_md"], update "bf2_key" (eval_val_to_sval (ValBaseBit
+                (P4Arith.to_lbool ipv4_addr_w (snd h) ++ P4Arith.to_lbool ipv4_addr_w (fst h))))
+          (update "bf2_api" (P4Bit 8 QUERY)
+            (update "solicited" (P4Bit 8 0)
+              (force ValBaseNull (uninit_sval_of_typ None metadata_t)))))]
+        (EXT []))).
+
+Lemma bf2_act_set_query_key_body : 
+  func_sound ge bf2_act_set_query_key_fd nil bf2_act_set_query_key_spec.
+Proof.
+  start_function.
+  step.
+  step.
+  step.
+  entailer.
+Qed.
+
+#[local] Hint Extern 5 (func_modifies _ _ _ _ _) => (apply bf2_act_set_query_key_body) : func_specs.
+
+Definition bf2_tbl_set_key_fd :=
+  ltac:(get_fd ["SwitchIngress"; "bf2_tbl_set_key"; "apply"] ge).
+
+Definition bf2_tbl_set_key_spec :=
+  WITH (* p *),
+    PATH p
+    MOD (Some [["ig_md"]; ["bf2_act_set_insert_key"; "api"]; ["bf2_act_set_query_key"; "api"]]) []
+    WITH h,
+      PRE
+        (ARG []
+        (MEM [(["hdr"], update "ipv4"
+                (update "src_addr" (P4Bit ipv4_addr_w (fst h))
+                  (update "dst_addr" (P4Bit ipv4_addr_w (snd h))
+                    (force ValBaseNull (uninit_sval_of_typ (Some true) ipv4_h))))
+                (force ValBaseNull (uninit_sval_of_typ None header_t)));
+              (["ig_md"], update "solicited" (P4Bit 8 0)
+                (force ValBaseNull (uninit_sval_of_typ None metadata_t)))]
+        (EXT [])))
+      POST
+      (EX retv,
+        (ARG_RET [] retv
+        (MEM [(["ig_md"], update "bf2_key" (eval_val_to_sval (ValBaseBit
+              (if is_internal (fst h) then
+                P4Arith.to_lbool ipv4_addr_w (fst h) ++ P4Arith.to_lbool ipv4_addr_w (snd h)
+               else
+                P4Arith.to_lbool ipv4_addr_w (snd h) ++ P4Arith.to_lbool ipv4_addr_w (fst h))))
+          (update "bf2_api" (P4Bit 8 (if is_internal (fst h) then INSERT else QUERY))
+            (update "solicited" (P4Bit 8 0)
+              (force ValBaseNull (uninit_sval_of_typ None metadata_t)))))]
+        (EXT []))))%arg_ret_assr.
+
+Lemma bf2_tbl_set_key_body :
+  func_sound ge bf2_tbl_set_key_fd nil bf2_tbl_set_key_spec.
+Proof.
+  start_function.
+  - change (is_true (is_internal (fst h))) in H.
+    replace (is_internal (fst h)) with true by auto.
+    table_action bf2_act_set_insert_key_body.
+    { entailer. }
+    { entailer. }
+  - change (is_true (~~is_internal (fst h))) in H.
+    replace (is_internal (fst h)) with false. 2 : {
+      destruct (is_internal (fst h)); auto; inv H.
+    }
+    table_action bf2_act_set_query_key_body.
+    { entailer. }
+    { entailer. }
+  - elim_trivial_cases.
+Qed.
+
+#[local] Hint Extern 5 (func_modifies _ _ _ _ _) => (apply bf2_tbl_set_key_body) : func_specs.
+
+Definition act_for_tbl_3_action_0_fd :=
+  ltac:(get_fd ["SwitchIngress"; "act_for_tbl_3_action_0"] ge).
+
+Definition act_for_tbl_3_action_0_spec :=
+  WITH (* p *),
+    PATH p
+    MOD (Some [["ig_intr_dprsr_md"]]) []
+    WITH ,
+      PRE
+        (ARG []
+        (MEM [(["ig_intr_dprsr_md"],
+                (force ValBaseNull (uninit_sval_of_typ None ingress_intrinsic_metadata_for_deparser_t)))]
+        (EXT [])))
+      POST
+        (ARG_RET [] ValBaseNull
+        (MEM [(["ig_intr_dprsr_md"], update "drop_ctl" (P4Bit 3 1)
+                (force ValBaseNull (uninit_sval_of_typ None ingress_intrinsic_metadata_for_deparser_t)))]
+        (EXT []))).
+
+Lemma act_for_tbl_3_action_0_body :
+  func_sound ge act_for_tbl_3_action_0_fd nil act_for_tbl_3_action_0_spec.
+Proof.
+  start_function.
+  step.
+  step.
+  entailer.
+Qed.
+
+Definition act_for_tbl_3_action_1_fd :=
+  ltac:(get_fd ["SwitchIngress"; "act_for_tbl_3_action_1"] ge).
+
+Definition act_for_tbl_3_action_1_spec :=
+  WITH (* p *),
+    PATH p
+    MOD (Some [["ig_intr_dprsr_md"]]) []
+    WITH ,
+      PRE
+        (ARG []
+        (MEM [(["ig_intr_dprsr_md"],
+                (force ValBaseNull (uninit_sval_of_typ None ingress_intrinsic_metadata_for_deparser_t)))]
+        (EXT [])))
+      POST
+        (ARG_RET [] ValBaseNull
+        (MEM [(["ig_intr_dprsr_md"], update "drop_ctl" (P4Bit 3 0)
+                (force ValBaseNull (uninit_sval_of_typ None ingress_intrinsic_metadata_for_deparser_t)))]
+        (EXT []))).
+
+Lemma act_for_tbl_3_action_1_body :
+  func_sound ge act_for_tbl_3_action_1_fd nil act_for_tbl_3_action_1_spec.
+Proof.
+  start_function.
+  step.
+  step.
+  entailer.
+Qed.
+
+Definition tbl_for_stmt_3_fd :=
+  ltac:(get_fd ["SwitchIngress"; "tbl_for_stmt_3"; "apply"] ge).
+
+Definition tbl_for_stmt_3_spec :=
+  WITH (* p *),
+    PATH p
+    MOD (Some [["ig_intr_dprsr_md"]]) []
+    WITH solicited,
+      PRE
+        (ARG []
+        (MEM [(["ig_md"], update "solicited" (P4Bit_option 8 (option_map Z.b2z solicited))
+                (force ValBaseNull (uninit_sval_of_typ None metadata_t)));
+              (["ig_intr_dprsr_md"],
+                (force ValBaseNull (uninit_sval_of_typ None ingress_intrinsic_metadata_for_deparser_t)))]
+        (EXT [])))
+      POST
+      (EX retv,
+        (ARG_RET [] retv
+        (MEM [(["ig_intr_dprsr_md"], update "drop_ctl" (P4Bit_option 3 (option_map Z.b2z (option_map negb solicited)))
+                (force ValBaseNull (uninit_sval_of_typ None ingress_intrinsic_metadata_for_deparser_t)))]
+        (EXT []))))%arg_ret_assr.
+
+Lemma tbl_for_stmt_3_body :
+  func_sound ge tbl_for_stmt_3_fd nil tbl_for_stmt_3_spec.
+Proof.
+  start_function.
+  - table_action act_for_tbl_3_action_0_body.
+    { entailer. }
+    { entailer.
+      destruct solicited as [[] | ].
+      - simpl in H2.
+        revert H.
+        simpl_sval_to_val.
+        intro H.
+        simpl_match_cond H.
+        inv H.
+      - repeat constructor.
+      - repeat constructor.
+    }
+  - table_action act_for_tbl_3_action_1_body.
+    { entailer. }
+    { entailer.
+      destruct solicited as [[] | ].
+      - repeat constructor.
+      - simpl in H2.
+        revert H.
+        simpl_sval_to_val.
+        intro H.
+        simpl_match_cond H.
+        inv H.
+      - repeat constructor.
+    }
+  - elim_trivial_cases.
+Qed.
+
+#[local] Hint Extern 5 (func_modifies _ _ _ _ _) => (apply tbl_for_stmt_3_body) : func_specs.
 
 Definition Ingress_fd :=
   ltac:(get_fd ["SwitchIngress"; "apply"] ge).
@@ -46,10 +352,11 @@ Definition Ingress_spec : func_spec :=
         (ARG [update "ipv4"
                 (update "src_addr" (P4Bit ipv4_addr_w (fst h))
                   (update "dst_addr" (P4Bit ipv4_addr_w (snd h))
-                    (force ValBaseNull (uninit_sval_of_typ None ipv4_h))))
+                    (force ValBaseNull (uninit_sval_of_typ (Some true) ipv4_h))))
                 (force ValBaseNull (uninit_sval_of_typ None header_t));
               force ValBaseNull (uninit_sval_of_typ None metadata_t);
-              force ValBaseNull (uninit_sval_of_typ None ingress_intrinsic_metadata_t);
+              update "ingress_mac_tstamp" (P4Bit 48 tstamp)
+                (force ValBaseNull (uninit_sval_of_typ (Some true) ingress_intrinsic_metadata_t));
               force ValBaseNull (uninit_sval_of_typ None ingress_intrinsic_metadata_from_parser_t);
               force ValBaseNull (uninit_sval_of_typ None ingress_intrinsic_metadata_for_deparser_t);
               force ValBaseNull (uninit_sval_of_typ None ingress_intrinsic_metadata_for_tm_t)
@@ -60,7 +367,7 @@ Definition Ingress_spec : func_spec :=
         (ARG_RET [update "ipv4"
                     (update "src_addr" (P4Bit ipv4_addr_w (fst h))
                       (update "dst_addr" (P4Bit ipv4_addr_w (snd h))
-                        (force ValBaseNull (uninit_sval_of_typ None ipv4_h))))
+                        (force ValBaseNull (uninit_sval_of_typ (Some true) ipv4_h))))
                     (force ValBaseNull (uninit_sval_of_typ None header_t));
                   force ValBaseNull (uninit_sval_of_typ None metadata_t);
                   update "drop_ctl" (P4Bit_option 3 (option_map Z.b2z (snd (process f (tstamp, h)))))
@@ -74,4 +381,41 @@ Lemma Ingress_body :
   func_sound ge Ingress_fd nil Ingress_spec.
 Proof.
   start_function.
-Admitted.
+  step_call tbl_for_stmt_1_body.
+  { entailer. }
+  Intros _.
+  step_call bf2_tbl_set_key_body.
+  { entailer. }
+  Intros _.
+  destruct (is_internal (fst h)) eqn:H_is_internal.
+  - step_call Filter_insert_body (fst h, snd h) tstamp.
+    { entailer. }
+    step_call tbl_for_stmt_3_body (Some false).
+    { entailer.
+      repeat constructor.
+    }
+    Intros _.
+    step.
+    unfold process.
+    rewrite H_is_internal.
+    destruct h.
+    entailer.
+    repeat constructor.
+  - step_call Filter_query_body (snd h, fst h) tstamp.
+    { entailer.
+      repeat constructor.
+    }
+    step_call tbl_for_stmt_3_body (filter_query (filter_clear f tstamp) (tstamp, (snd h, fst h))).
+    { entailer.
+      repeat constructor.
+      apply sval_refine_refl.
+    }
+    Intros _.
+    step.
+    unfold process.
+    rewrite H_is_internal.
+    destruct h.
+    entailer.
+    + destruct (filter_query (filter_clear f tstamp) (tstamp, _));
+      repeat constructor.
+Qed.
