examples/sbf/flow_proof.v
@@ -1,0 +1,444 @@
+Require Import VST.floyd.proofauto.
+Require Import ProD3.examples.sbf.common.
+Require Import ProD3.examples.sbf.LightFilter.
+Require Import ProD3.examples.sbf.verif_Filter_all.
+Require Import ProD3.examples.sbf.verif_Ingress.
+Definition Time:= Z.
+
+Definition ip_addr := Z.
+(* Parameter ip_addrDummy: Inhabitant ip_addr. *)
+(* Parameter T Tc:Time. *)
+Notation T := (T num_frames frame_time).
+Notation Tc := (Tc num_slots frame_time).
+(* Parameter is_internal: ip_addr -> bool. *)
+
+(* Parameter filter_base : Type. *)
+
+(* Record Header := { SrcAddr: ip_addr; DstAddr : ip_addr }. *)
+Definition Header : Type := Z * Z.
+Definition Build_Header : Z -> Z -> Header := pair.
+Definition SrcAddr : Header -> Z := fst.
+Definition DstAddr : Header -> Z := snd.
+
+(* Definition DefaultHeader:Inhabitant Header. split. apply ip_addrDummy.  apply ip_addrDummy. Defined. *)
+
+Definition insert : filter -> Time * Header -> filter :=
+  filter_insert.
+
+Definition query : filter -> Time * Header -> option bool :=
+  filter_query.
+
+Definition clear : filter -> Time -> filter :=
+  filter_clear.
+
+Opaque insert query clear.
+
+(* Parameter insert : (option filter_base) -> (Time * Header) -> (option filter_base).
+Parameter query : (option filter_base) -> (Time * Header) -> option bool.
+Parameter clear : (option filter_base) -> Time -> (option filter_base). *)
+Parameter empty : Time -> filter.
+Parameter ok_until: filter -> Time -> Prop.
+
+Axiom query_clear: forall f t t' h,
+  t <= t' ->
+  ok_until f t ->
+  query f (t', h) = query (clear f t) (t', h).
+
+Axiom query_insert_same : forall f t t' h,
+  t <= t' <= t+T ->
+  ok_until f t ->
+  query (insert f (t, h)) (t', h) = Some true.
+
+Axiom query_insert_other : forall f t t' h h',
+  t <= t' ->
+  ok_until f t ->
+  query f (t', h') = Some true ->
+  query (insert f (t, h)) (t', h') = Some true.
+
+Axiom ok_insert: forall f t t' h, t <= t' <= t+Tc -> ok_until f t ->
+             ok_until (insert f (t,h)) t'.
+
+Axiom ok_clear: forall f t t', t <= t' <= t+Tc -> ok_until f t ->
+            ok_until (clear f t) t'.
+
+Axiom empty_ok: forall t, ok_until (empty t) t.
+
+Definition Payload := list bool.
+(* Definition DummyData: Inhabitant Payload.
+  typeclasses eauto.
+  unfold Payload.  *)
+
+Definition Packet:Type := (Time * Header) * Payload.
+Definition Result:Type := option (Header * Payload).
+
+Definition FirewallState:Type := filter.
+
+Inductive fw_process_packet: FirewallState -> Packet -> FirewallState -> Result -> Prop :=
+| fw_outgoing: forall f t h data, is_internal (SrcAddr h) = true ->
+               fw_process_packet f ((t,h),data) (insert f (t, h)) (Some (h, data))
+
+(*Incoming packet is permitted by the firewall*)
+| fw_incomingPermit: forall f t h data, is_internal (SrcAddr h) = false ->
+               In (query (clear f t) (t, Build_Header (DstAddr h) (SrcAddr h)))
+                  [None; Some true] ->
+               fw_process_packet f ((t,h),data) (clear f t) (Some (h, data))
+
+(*this is the case where packets are dropped, ie DOS is detected*)
+| fw_incomingDrop: forall f t h data, is_internal (SrcAddr h) = false -> 
+               In (query (clear f t)  (t, Build_Header (DstAddr h) (SrcAddr h)))
+                  [ None; Some false] ->
+               fw_process_packet f ((t,h),data) (clear f t) None.
+
+Inductive trans_fw: FirewallState -> list Packet -> FirewallState -> list Result -> Prop :=
+  trans_nil: forall f, trans_fw f [] f []
+|
+  trans_step: forall f h k u, trans_fw f h k u -> forall p g r,
+                fw_process_packet k p g r -> trans_fw f (h++[p]) g (u++[r]).
+
+Lemma trans_single: forall f p g r, fw_process_packet f p g r -> trans_fw f [p] g [r].
+Proof. intros. simpl. eapply (trans_step f [] f []). constructor. trivial. Qed.
+
+Lemma trans_cons: forall f p g r, fw_process_packet f p g r ->
+                  forall h k u, trans_fw g h k u -> 
+                trans_fw f (p::h) k (r::u).
+Proof. intros. induction H0; simpl; intros.
++ eapply trans_single. trivial.
++ replace (p :: h ++ [p0]) with ((p :: h) ++ [p0]) by reflexivity.
+  replace (r :: u ++ [r0]) with ((r :: u) ++ [r0]) by reflexivity.
+  eapply trans_step; eauto.
+Qed.
+
+Lemma trans_app_inv: forall l2 {l f g r}, trans_fw f l g r ->
+      forall l1, l=l1++l2 ->
+      exists k r1 r2,
+       trans_fw f l1 k r1  /\ trans_fw k l2 g r2 /\ r=r1++r2.
+Proof. induction l2; simpl; intros.
++ rewrite app_nil_r in H0; subst l1.
+  do 3 eexists; split3. eauto. apply trans_nil. rewrite app_nil_r; trivial.
++ specialize (IHl2 _ _ _ _ H (l1 ++ [a])). rewrite <- app_assoc in IHl2.
+  destruct (IHl2 H0) as [k [r1 [r2 [T1 [T2 R]]]]]; clear IHl2 H. subst.
+  inv T1. 1: symmetry in H1; apply app_eq_nil in H1; destruct H1; congruence.
+  apply app_inj_tail in H. destruct H; subst h p.
+  do 3 eexists; split3.
+  - eassumption.
+  - eapply trans_cons. apply H2. apply T2.
+  - rewrite <- app_assoc; trivial.
+Qed.
+
+Lemma trans_cons_inv: forall h l f g r, trans_fw f l g r ->
+      forall p, l=p::h ->
+      exists k r1 r2,
+       fw_process_packet f p k r1 /\ trans_fw k h g r2 /\ r=r1::r2.
+Proof. intros.
+  destruct (trans_app_inv h H [p] H0) as [k [r1 [r2 [P [HH R]]]]].
+  clear H; inv P. destruct h0; inv H; [ | apply app_eq_nil in H4; destruct H4; congruence].
+  inv H1; simpl.
+  + do 3 eexists; split3; eauto.
+  + apply app_eq_nil in H; destruct H; congruence.
+Qed.
+
+Definition get_tstamp (p : Packet) : Time := (fst (fst p)).
+
+Definition get_src (p : Packet) : ip_addr := SrcAddr (snd (fst p)).
+
+Definition get_dst (p : Packet) : ip_addr := DstAddr (snd (fst p)).
+
+Lemma fw_packet_preserves_okUntil {f p g r}:
+      fw_process_packet f p g r -> let t:= get_tstamp p in 
+      ok_until f t -> forall t', t <= t' <= t+Tc -> ok_until g t'.
+Proof. induction 1; unfold get_tstamp; simpl; intros.
++ (*fw_outgoingSuccess*) apply ok_insert; trivial.
++ (*fw_incomingPermit*) apply ok_clear; trivial.
++ (*fw_incomingDrop*) apply ok_clear; trivial.
+Qed.
+
+(* #[global] Instance d:Inhabitant Packet. split. split. apply 0. apply DefaultHeader.  Defined. *)
+
+Definition recent p q T := 0 <= get_tstamp p - get_tstamp q < T. (*NEW: I require that difference always be nonneg. Maybe that's not necessary*)
+
+Definition valid_flow (f : list Packet) :=
+  forall i, 0 <= i < Zlength f - 1 -> recent (Znth  (i + 1) f) (Znth i f) Tc.
+
+Lemma valid_flow_cons_inv {l p}: valid_flow (p::l) -> valid_flow l.
+Proof. unfold valid_flow; intros. rewrite Zlength_cons in H.
+  exploit (H (i+1)); clear H; intros. lia. rewrite 2 Znth_pos_cons in H by lia.
+  replace (i + 1 + 1 - 1) with (i + 1) in H by lia.
+  replace (i + 1 - 1) with i in H by lia. apply H.
+Qed.
+Lemma valid_flow_app_inv {l}: forall {m}, valid_flow (l++m) -> valid_flow l /\ valid_flow m.
+Proof.
+  induction l; simpl; intros.
++ split; trivial. red. list_solve.
++ destruct (IHl _ (@valid_flow_cons_inv (l++m) a H)); clear IHl. split; trivial.
+  clear - H. red; intros. exploit (H i); clear H; list_solve.
+Qed.
+
+Lemma trans_preserves_okUntil {h}: valid_flow h -> h <> nil ->
+      forall f k u,
+      trans_fw f h k u -> 
+      let t0 := get_tstamp (Znth 0 h) in
+      ok_until f t0 -> forall t', 0 <= t' - get_tstamp (Znth (Zlength h-1) h) < Tc ->
+      ok_until k t'.
+Proof. intros ? ? ? ? ? ?. induction H1; intros. elim H0; trivial.
+destruct (valid_flow_app_inv H) as [ Hvalid _].
+specialize (IHtrans_fw Hvalid).
+destruct h as [| [hh ht]].
++ clear IHtrans_fw. inv H1; [ | list_solve].
+  apply (fw_packet_preserves_okUntil H2); subst t0; list_solve.
++ assert (X: (hh, ht) :: h <> []) by (clear; intros N; list_solve).
+  specialize (IHtrans_fw X H3).
+  apply (fw_packet_preserves_okUntil H2); clear H2.
+  - apply IHtrans_fw; clear IHtrans_fw. clear H4; subst t0.
+    clear H3. clear - H.
+    exploit (H (Zlength h)); clear H.
+     * list_solve.
+     * unfold Packet in *. 
+       replace ((@Zlength (Time * Header * Payload) h + 1
+                - @Zlength (Time * Header * Payload)  ((hh, ht) :: h)))
+       with 0 by list_solve.
+       replace (@Zlength (Time * Header * Payload)
+            ((hh, ht) :: h) - 1) 
+       with (@Zlength (Time * Header * Payload) h) by list_solve.
+       intros X; red in X; list_solve.
+   - clear- H4; unfold Packet in *.
+     replace (Zlength (((hh, ht) :: h) ++ [p]) - 1) with
+             (Zlength ((hh, ht) :: h)) in H4 by list_solve.
+      rewrite Znth_app2, Zminus_diag in H4 by list_solve.
+      rewrite Znth_0_cons in H4; lia.
+Qed. 
+
+Lemma valid_flow_trans_wf: forall f (Hf: valid_flow f) s
+      (Hs: match f with nil => True | hd::tl => ok_until s (get_tstamp hd) end),
+      exists t r, trans_fw s f t r.
+Proof. induction f; simpl; intros.
++ do 2 eexists. apply trans_nil.
++ assert (Ha: exists u r1, fw_process_packet s a u r1).
+  { clear IHf. destruct a as [[ta h] data].
+    remember (is_internal (SrcAddr h)) as dir; symmetry in Heqdir; destruct dir.
+    - do 2 eexists. apply fw_outgoing. trivial.
+    - remember (query (clear s ta) (ta, Build_Header (DstAddr h) (SrcAddr h))) as q; destruct q.
+      * destruct b.
+        { specialize (fw_incomingPermit s ta h data Heqdir).
+          rewrite <- Heqq. intros X. do 2 eexists.
+          apply X. right; left; trivial. }
+        { specialize (fw_incomingDrop s ta h data Heqdir).
+          rewrite <- Heqq. intros X. do 2 eexists.
+          apply X. right; left; trivial. }
+      * specialize (fw_incomingDrop s ta h data Heqdir).
+          rewrite <- Heqq. intros X. do 2 eexists.
+          apply X. left; trivial. }
+  destruct Ha as [u [r1 HHa]]. 
+  destruct (IHf (valid_flow_cons_inv Hf) u) as [t [r2 HHf]].
+  - clear IHf. destruct f; trivial. apply trans_single in HHa.
+    assert (Va: valid_flow [a]) by (red; intros; list_solve).
+    assert (Xa: [a] <> []) by congruence. 
+    apply (@trans_preserves_okUntil [a] Va Xa _ _ _ HHa Hs).
+    exploit (Hf 0); clear Hf. list_solve. simpl.
+    intros R; apply R.
+  - exists t, (r1::r2). eapply trans_cons; eassumption.
+Qed.
+
+Definition high_level_exec (h : list Packet) (p : Packet) (res : Result) :=
+  exists h' f g,
+    trans_fw (empty (get_tstamp (Znth 0 (h++[p])))) h f h' /\
+    fw_process_packet f p g res.
+
+Definition property (h : list Packet) (p : Packet) (res : Result) : Prop :=
+    is_internal (get_src p) = false /\ is_internal (get_dst p) = true /\
+    (exists i, 0 <= i < Zlength h /\ recent p (Znth i h) T /\
+      get_src p = get_dst (Znth i h) /\ get_dst p = get_src (Znth i h)) ->
+  isSome res.
+
+Lemma list_nil_or_snoc {A}: forall (l:list A),
+       l=[] \/ exists l1 a, l=l1++[a].
+Proof.
+  induction l; simpl; intros. left; trivial.
+  right. destruct IHl.
++ subst. exists [], a; trivial.
++ destruct H as [l1 [aa Hl]]; subst.
+  exists (a::l1), aa. trivial.
+Qed.
+
+Lemma flow_level_property : forall (h : list Packet) (p : Packet) (res : Result),
+  high_level_exec h p res ->
+  valid_flow (h ++ [p]) ->
+  property h p res.
+Proof. intros. red. intros [Hsrc [Hdst [i [Hi [iRecent [iSrc iDst]]]]]].
+destruct H as [result [f [g [Trans Step]]]].
+destruct p as [[tp header] data].
+
+inv Step; simpl; trivial.
+(*Interesting case: DROP*)
+unfold get_src, get_dst in *. simpl in *. clear H6. 
+destruct header as [sH dH]; simpl in *.
+assert (OK_f: ok_until f tp).
+{ destruct (valid_flow_app_inv H0).
+  eapply (trans_preserves_okUntil H). 
+     + intros N; subst; list_solve.
+     + apply Trans.
+     + rewrite Znth_app1 by list_solve. apply empty_ok.
+     + clear - Hi H0. exploit (H0 (Zlength h -1)). list_solve.
+        replace (Zlength h - 1 + 1) with (Zlength h) by list_solve.
+        intros R; red in R. unfold get_tstamp in *.
+        rewrite Znth_app2, Zminus_diag, Znth_0_cons in R by lia. simpl in R.
+        rewrite Znth_app1 in R by list_solve; trivial. }
+assert (query (clear f tp)
+              (tp, Build_Header dH sH) = Some true);
+[ 
+|rewrite H in H7; destruct H7 as [Q | [ Q | Q]]; congruence; contradiction].
+clear H7.
+erewrite <- query_clear; trivial. 2:lia. unfold Packet in *. 
+remember ((h ++
+                    [(tp, ((sH, dH) : Header),
+                     data)])) as l in *.
+
+exploit (split3_full_length_list 0 i (Zlength h) h Hi). lia.
+rewrite Zminus_0_r; intros Hh.
+assert (exists state1 res1 state2 resI res2, 
+  trans_fw (empty (get_tstamp (Znth 0 l)))  (firstn (Z.to_nat i) h) state1 res1 /\
+  fw_process_packet state1 (Znth i h) state2 resI /\
+  trans_fw state2 (skipn (Z.to_nat (i + 1)) h) f res2 /\
+  result = res1++resI::res2 /\ state2 = insert state1 (fst (Znth i h))).
+{ clear- Hh Trans iDst iSrc Hdst Hsrc. (*symmetry in Hh.*) rewrite app_assoc in Hh.
+  destruct (trans_app_inv _ Trans _ Hh)
+  as [ state1 [res1 [res2 [Trans1 [Trans2 R]]]]]. subst.
+  inv Trans1. { symmetry in H1. apply app_eq_nil in H1; destruct H1; congruence. }
+  apply app_inj_tail in H. destruct H; subst h0 p.
+  do 5 eexists; split3. eassumption. eassumption.
+  split3. eassumption. rewrite <- app_assoc. trivial.
+  inv H2. + trivial.
+    + rewrite <- H in *;  simpl in *. congruence.
+    + rewrite <- H in *;  simpl in *. congruence. }
+
+destruct H as [state1 [res1 [state2 [resI [res2 [Front [StepI [Tail [R HState2]]]]]]]]].
+clear Trans. 
+
+assert(ValidFrontI: valid_flow ((firstn (Z.to_nat i) h) ++ [Znth i h])).
+{ subst l. destruct (valid_flow_app_inv H0). clear - H Hh.
+  rewrite Hh, app_assoc in H. apply (valid_flow_app_inv H). }
+assert(ValidFront: valid_flow (firstn (Z.to_nat i) h)) by 
+  apply (valid_flow_app_inv ValidFrontI).
+assert(ValidITail: valid_flow ([Znth i h] ++ skipn (Z.to_nat (i + 1)) h)).
+{ subst l. destruct (valid_flow_app_inv H0). clear - H Hh.
+  rewrite Hh in H. apply (valid_flow_app_inv H). }
+assert (ValidTail: valid_flow (skipn (Z.to_nat (i + 1)) h)) by apply (valid_flow_app_inv ValidITail).
+forget (skipn (Z.to_nat (i + 1)) h) as tail.
+
+assert (Hstate2: state2 = insert state1 (fst (Znth i h))).
+{ clear Front. inv StepI; rewrite <- H in *; trivial. }
+
+assert (State1OK: ok_until state1 (get_tstamp (Znth i h))).
+{ clear - ValidFrontI Front ValidFront Hi Heql.
+  remember (firstn (Z.to_nat i) h) as front; destruct front.
+  + inv Front.
+    - destruct h. list_solve. simpl in *.
+      remember (Z.to_nat i) as n; destruct n; simpl in Heqfront; [ | discriminate].
+      assert (i=0) by lia; subst i. clear. (* clear H1 Hi Heqn; simpl in *.*)
+      rewrite ! Znth_0_cons. apply empty_ok.
+    - apply app_eq_nil in H; destruct H; congruence.
+  + assert (HF: (p::front) <> []) by congruence. (* (rewrite <- H; intros N; apply app_eq_nil in N; destruct N; congruence).*)
+    specialize (trans_preserves_okUntil ValidFront HF _ _ _ Front). subst l. simpl. rewrite ! Znth_0_cons. intros H.
+    apply H; clear H Front.
+    * destruct h; simpl.
+      - destruct (Z.to_nat i); simpl in Heqfront; congruence.
+      - rewrite Znth_0_cons; simpl. 
+        remember (Z.to_nat i) as n; destruct n; simpl in *; inv Heqfront. 
+        apply empty_ok.
+    * red in ValidFrontI.
+      exploit (ValidFrontI (Zlength front)).
+      - unfold Packet in *; list_solve. 
+      - clear - HF. replace (Znth (Zlength front + 1) ((p :: front) ++ [Znth i h])) with (Znth i h) by list_solve.
+        replace (Znth (Zlength front) ((p :: front) ++ [Znth i h]))
+        with (Znth (Zlength (p :: front) - 1) (p :: front)) by list_solve.
+        trivial. }
+
+assert (State2OK: forall t', 0 <= t' - get_tstamp (Znth i h) < Tc ->
+      ok_until state2 t').
+1: intros; apply (fw_packet_preserves_okUntil StepI); [ trivial | lia].
+
+clear Front.
+forget (firstn (Z.to_nat i) h) as front.
+clear ValidFront StepI. 
+assert (ValidTailTp: valid_flow (tail++[(tp, ((sH, dH) : Header), data)])).
+{ clear - Hh Heql H0. subst l.  rewrite Hh in H0. 
+  rewrite <- app_assoc in H0. 
+  apply valid_flow_app_inv in H0. destruct H0 as [_ HH].
+  rewrite <- app_assoc in HH. 
+  apply (valid_flow_app_inv HH). }
+assert (QI: query (insert state1 (fst (Znth i h)))
+   (tp, ((dH, sH) : Header)) = Some true).
+{ subst sH dH. destruct (Znth i h). simpl in *.
+  destruct p; simpl in *. destruct h0. simpl in *. apply query_insert_same.
+  + simpl in *.
+    clear - iRecent. red in iRecent. unfold get_tstamp in *. simpl in *. lia.
+  + apply State1OK. }
+rewrite <- Hstate2 in *.  
+clear - ValidITail State2OK ValidTailTp Tail QI iRecent.
+forget (Znth i h) as packetI.
+(*rewrite <- H2; clear H2.*)
+unfold Build_Header in *.
+forget (dH, sH) as headerP.
+forget (sH, dH) as headerI.
+clear sH dH h.
+generalize dependent packetI.
+
+ (*generalize dependent tp.*) generalize dependent res2. generalize dependent f.
+generalize dependent state2. 
+induction tail; intros.
++ inv Tail. trivial. apply app_eq_nil in H; destruct H; congruence.
++ destruct (@trans_cons_inv tail (a :: tail) _ _ _ Tail _ (eq_refl _))
+  as [k [resA [resB [FwA [TransB RES]]]]]; clear Tail.
+  assert (VF: valid_flow
+           (tail ++ [(tp, headerI, data)])). 
+  { replace (a :: tail) with ([a]++tail) in ValidTailTp by reflexivity.
+    rewrite <- app_assoc in ValidTailTp. apply (valid_flow_app_inv ValidTailTp). }
+  assert (Ht_packetI: 0 <= get_tstamp a - get_tstamp packetI < Tc).
+  { exploit (ValidITail 0). unfold Packet in *; list_solve. 
+    simpl. rewrite Znth_pos_cons, Zminus_diag, ! Znth_0_cons by list_solve.
+    intros H; apply H. } 
+  assert(OK_g_a: ok_until state2 (get_tstamp a)).
+  { apply State2OK; trivial. }
+  assert (H_a_tp: (get_tstamp a) <= tp).
+  { clear - ValidTailTp. generalize dependent a. induction tail; simpl; intros.
+    ** exploit (ValidTailTp 0); clear ValidTailTp. unfold Packet in *; list_solve.
+       simpl. unfold recent; intros. unfold get_tstamp in *.
+       rewrite Znth_pos_cons, Zminus_diag, ! Znth_0_cons in H. simpl in H. lia. lia. 
+    ** unfold Header in *.
+       replace (a0 :: a :: tail ++ [(tp, headerI, data)]) with ([a0] ++ ( a :: tail ++ [(tp, headerI, data)])) in ValidTailTp by reflexivity.
+       destruct (valid_flow_app_inv ValidTailTp).
+       apply IHtail in H0; clear IHtail.
+       replace ([a0] ++ a :: tail ++ [(tp, headerI, data)]) 
+           with (([a0;a] ++ (tail ++ [(tp, headerI, data)]))) in ValidTailTp by reflexivity.
+       destruct (valid_flow_app_inv ValidTailTp).
+       exploit (H1 0); clear - H0. unfold Packet, Header in *; list_solve.
+       simpl. rewrite Znth_pos_cons, Zminus_diag, ! Znth_0_cons by list_solve. intros.
+       red in H.  unfold get_tstamp in *. lia. }
+  assert (Hk: query k (tp, headerP) = Some true).
+  { clear IHtail TransB.
+    inv FwA.
+    + apply query_insert_other; trivial.
+    + rewrite <- query_clear; trivial.
+    + rewrite <- query_clear; trivial. }
+  apply (IHtail VF _ Hk  _ _ TransB a); clear IHtail.
+  - clear - iRecent ValidITail ValidTailTp H_a_tp. red.
+    red in iRecent. exploit (ValidITail 0); clear ValidITail; simpl. unfold Packet in *; list_solve.
+    intros. rewrite Znth_pos_cons,Zminus_diag, ! Znth_0_cons in H by list_solve.
+    red in H. unfold get_tstamp in *. simpl in *; lia.
+  - apply (valid_flow_app_inv ValidITail).
+  - specialize (fw_packet_preserves_okUntil FwA). intros. apply H; clear H.
+    * trivial.
+    * lia.
+Qed.
+
+Lemma full_property h p (Vp: valid_flow (h ++ [p])):
+  (exists res, high_level_exec h p res) /\
+  (forall res, high_level_exec h p res -> property h p res).
+Proof. destruct (valid_flow_trans_wf _ Vp (empty (get_tstamp (Znth 0 (h++[p]))))) as [t [r Hr]].
+  + destruct h; simpl; apply empty_ok.
+  + split.
+    - unfold high_level_exec. inv Hr.
+      * symmetry in H1; apply app_eq_nil in H1; destruct H1; congruence.
+      * apply app_inj_tail in H. destruct H; subst p0 h0.
+        do 4 eexists. split; eassumption.
+    - intros. eapply flow_level_property; trivial.
+Qed.
