examples/sbf/verif_switch.v
@@ -1,0 +1,120 @@
+Require Import Coq.ZArith.BinInt.
+Require Import Coq.Program.Program.
+Require Poulet4.Utils.Utils.
+Require Import Coq.NArith.BinNat.
+Require Import Poulet4.P4light.Syntax.P4defs.
+Require Import Poulet4.P4light.Semantics.Semantics.
+Require Import ProD3.core.Core.
+Require Import ProD3.core.Tofino.
+Require Import ProD3.examples.sbf.Utils.
+Require Import ProD3.examples.sbf.common.
+Require Import ProD3.examples.sbf.P4_types.
+Require Import ProD3.examples.sbf.verif_Filter_all.
+Require Import ProD3.examples.sbf.verif_Ingress.
+Require Import ProD3.examples.sbf.flow_proof.
+Require Import ProD3.examples.sbf.switch.
+Require Import Hammer.Plugin.Hammer.
+
+Notation filter_repr := (filter_repr ["pipe"; "ingress"; "bf2_ds"]).
+
+Lemma inv_Forall2 : forall A B (P : A -> B -> Prop) a al b bl,
+  Forall2 P (a :: al) (b :: bl) ->
+  P a b /\ Forall2 P al bl.
+Proof.
+  inversion 1; auto.
+Qed.
+(* sval_refine_to_loptbool_eq *)
+Lemma sval_refine_P4Bit_eq : forall w v v',
+  sval_refine (P4Bit w v) v' ->
+  (P4Bit w v) = v'.
+Admitted.
+
+Lemma process_packet_fw_process_packet : forall es f p es' r,
+  filter_repr f es ->
+  process_packet ge P4_types.metadata_t es p es' r ->
+  exists f',
+    filter_repr f' es' /\ fw_process_packet f p f' r.
+Proof.
+  intros * H_filter_repr H_process_packet.
+  destruct p as [[tstamp h] payload].
+  exists (fst (process f (tstamp, h))).
+  inversion H_process_packet.
+  (* deal with function lookup *)
+  inv H2. inv H3. inv H4.
+  eapply (proj1 Ingress_body h) in H5.
+  2 : {
+    split.
+    { (* ARG *)
+      constructor.
+      { apply sval_refine_refl. }
+      constructor.
+      { apply sval_refine_refl. }
+      constructor.
+      { apply sval_refine_refl. }
+      constructor.
+      { apply sval_refine_refl. }
+      constructor.
+      { apply sval_refine_refl. }
+      constructor.
+      { apply sval_refine_refl. }
+      constructor.
+    }
+    split.
+    { (* MEM *)
+      constructor.
+    }
+    { (* EXT *)
+      constructor.
+      { apply H_filter_repr. }
+      constructor.
+    }
+  }
+  destruct H5 as [H_ARG [H_RET [H_MEM H_EXT]]].
+  split.
+  { inv H_EXT.
+    assumption.
+  }
+  apply inv_Forall2 in H_ARG.
+  destruct H_ARG as [H_hdr H_ARG].
+  apply inv_Forall2 in H_ARG.
+  destruct H_ARG as [H_ig_md H_ARG].
+  apply inv_Forall2 in H_ARG.
+  destruct H_ARG as [H_ig_intr_dprsr_md _].
+  replace (get "src_addr" (get "ipv4" hdr')) with (P4Bit ipv4_addr_w (fst h)) in *. 2 : {
+    clear -H_hdr.
+    pose proof (sval_refine_get _ _ "ipv4" H_hdr).
+    pose proof (sval_refine_get _ _ "src_addr" H).
+    rewrite get_update_same in H0 by auto.
+    rewrite get_update_same in H0 by auto.
+    apply sval_refine_P4Bit_eq in H0.
+    auto.
+  }
+  replace (get "dst_addr" (get "ipv4" hdr')) with (P4Bit ipv4_addr_w (snd h)) in *. 2 : {
+    clear -H_hdr.
+    pose proof (sval_refine_get _ _ "ipv4" H_hdr).
+    pose proof (sval_refine_get _ _ "dst_addr" H).
+    rewrite get_update_same in H0 by auto.
+    rewrite get_update_diff in H0 by (auto; congruence).
+    rewrite get_update_same in H0 by auto.
+    apply sval_refine_P4Bit_eq in H0.
+    auto.
+  }
+  replace ipv4' with h in *. 2 : {
+    admit.
+  }
+  assert (H_drop_ctl : bit_refine (snd (process f (tstamp, h))) (Some drop_ctl)). {
+    clear -H_ig_intr_dprsr_md.
+    pose proof (sval_refine_get _ _ "drop_ctl" H_ig_intr_dprsr_md).
+    rewrite get_update_same in H by auto.
+    change (snd (process f (tstamp, h))) with (snd (process f (tstamp, h))) in *.
+    destruct (snd (process f (tstamp, h))) as [[] | ].
+    - apply sval_refine_P4Bit_eq in H.
+      subst drop_ctl. rewrite <- H. constructor.
+    - apply sval_refine_P4Bit_eq in H.
+      subst drop_ctl. rewrite <- H. constructor.
+    - constructor.
+  }
+  unfold process in H_drop_ctl.
+  destruct (is_internal (fst h)) eqn:H_is_internal.
+  - inv H_drop_ctl.
+Admitted.
